concurrency/disciplined/sharedexclusive-linearatomic/GhostLinearSequence.i.dfy
@@ -1,0 +1,55 @@
+include "GhostLinearSequence.s.dfy"
+
+module GhostLinearSequence_i {
+  import opened GhostLinearMaybe
+  import opened GhostLinearSequence_s
+
+  function glseqs<A>(l:glseq<A>):(s:seq<A>)
+    ensures rank_is_less_than(s, l)
+    ensures |s| == |glseqs_raw(l)|
+  {
+    var s := seq(|glseqs_raw(l)|, i requires 0 <= i < |glseqs_raw(l)| => read(glseqs_raw(l)[i]));
+    axiom_glseqs_rank(l, s);
+    s
+  }
+
+  function operator(| |)<A>(s:glseq<A>):nat
+  {
+    |glseqs(s)|
+  }
+
+  function{:inline true} operator([])<A>(s:glseq<A>, i:nat):A
+      requires i < |s|
+  {
+    glseqs(s)[i]
+  }
+
+  function{:inline true} operator(in)<A>(s:glseq<A>, i:nat): bool
+    requires i < |s|
+  {
+    glseq_has(s)[i]
+  }
+
+  function method glseq_take<A>(glinear s1:glseq<A>, i:nat): (glinear p: (glinear glseq<A>, glinear A))
+      requires i < |s1| && i in s1
+      ensures p.1 == s1[i]
+      ensures glseq_has(p.0) == glseq_has(s1)[i := false]
+      ensures forall j:nat | j < |s1| && j != i as nat :: glseqs(p.0)[j] == glseqs(s1)[j]
+  {
+      glinear var x1:gmaybe<A> := empty();
+      glinear var (s2tmp, x2) := glseq_swap_raw(s1, i, x1);
+      (glinear s2tmp, glinear unwrap(x2))
+  }
+
+  function method glseq_give<A>(glinear s1: glseq<A>, i :nat, glinear a:A): (glinear s2: glseq<A>)
+      requires i < |s1|
+      requires i !in s1
+      ensures glseq_has(s2) == glseq_has(s1)[i := true]
+      ensures glseqs(s2) == glseqs(s1)[i := a]
+  {
+      glinear var x1:gmaybe<A> := give(a);
+      glinear var (s2tmp, x2) := glseq_swap_raw(s1, i, x1);
+      var _ := discard(x2);
+      s2tmp
+  }
+}
